theories/Syntax/BinOps.v
@@ -70,6 +70,7 @@ Module bop.
     | pair {σ1 σ2 : Ty} : BinOp σ1 σ2 (prod σ1 σ2)
     | cons {σ : Ty}     : BinOp σ (list σ) (list σ)
     | append {σ : Ty}   : BinOp (list σ) (list σ) (list σ)
+    | shiftr {m n}      : BinOp (bvec m) (bvec n) (bvec m)
     | bvadd {n}         : BinOp (bvec n) (bvec n) (bvec n)
     | bvsub {n}         : BinOp (bvec n) (bvec n) (bvec n)
     | bvmul {n}         : BinOp (bvec n) (bvec n) (bvec n)
@@ -98,6 +99,8 @@ Module bop.
       ((σ, list σ, list σ), cons).
     Definition binoptel_append (σ : Ty) : BinOpTel :=
       ((list σ, list σ, list σ), append).
+    Definition binoptel_shiftr (m n : nat) : BinOpTel :=
+      ((bvec m, bvec n, bvec m), shiftr).
 
     Definition is_eq {σ} (op : RelOp σ) : Datatypes.bool :=
       match op with eq => true | _ => false end.
@@ -153,6 +156,8 @@ Module bop.
         f_equal_dec binoptel_cons (ninv _ _) (eq_dec σ τ)
       | @append _ σ , @append _ τ   =>
         f_equal_dec binoptel_append (ninv _ _) (eq_dec σ τ)
+      | @shiftr _ m n , @shiftr _ p q =>
+          f_equal2_dec binoptel_shiftr (ninv _ _) (eq_dec m p) (eq_dec n q)
       | @bvadd _ m , @bvadd _ n =>
         f_equal_dec
           (fun n => ((bvec n, bvec n, bvec n), bvadd))
@@ -267,6 +272,7 @@ Module bop.
       | or         => fun v1 v2 => orb v1 v2
       | pair       => Datatypes.pair
       | cons       => List.cons
+      | shiftr     => fun v1 v2 => bv.shiftr v1 v2
       | append     => app
       | bvadd      => fun v1 v2 => bv.add v1 v2
       | bvsub      => fun v1 v2 => bv.sub v1 v2
